comment nonterminating proof, add more simple loop example

deps/poulet4/lib/P4automata/Examples/SimpleLoop.v
@@ -83,7 +83,7 @@ Module Loop.
 
 End Loop.
 
-Lemma prebisim_loop:
+(* Lemma prebisim_loop:
   pre_bisimulation (Sum.sum Loop.aut Loop.aut)
                    (WPSymLeap.wp (H:=_))
                    nil
@@ -135,4 +135,118 @@ Proof.
   solve_bisim'.
   cbv in *.
   intuition (try congruence).
-Time Qed.
+Time Qed. *)
+
+Module LoopUnroll.
+  Inductive state :=
+  | Start
+  | Second.
+  Scheme Equality for state.
+  Global Instance state_eqdec: EquivDec.EqDec state eq := state_eq_dec.
+  Global Program Instance state_finite: @Finite state _ state_eqdec :=
+    {| enum := [Start; Second] |}.
+  Next Obligation.
+    repeat constructor;
+      repeat match goal with
+             | H: List.In _ [] |- _ => apply List.in_nil in H; exfalso; exact H
+             | |- ~ List.In _ [] => apply List.in_nil
+             | |- ~ List.In _ (_ :: _) => unfold not; intros
+             | H: List.In _ (_::_) |- _ => inversion H; clear H
+             | _ => discriminate
+             end.
+  Qed.
+  Next Obligation.
+    destruct x; intuition congruence.
+  Qed.
+
+  Inductive header :=
+  | Var.
+
+  Global Instance hdr_eqdec: EquivDec.EqDec header eq.
+    vm_compute.
+    intros.
+    left.
+    destruct x; destruct x0; trivial.
+  Defined.
+  Global Program Instance header_finite: @Finite header _ hdr_eqdec :=
+    {| enum := [Var] |}.
+  Next Obligation.
+    repeat constructor;
+      repeat match goal with
+             | H: List.In _ [] |- _ => apply List.in_nil in H; exfalso; exact H
+             | |- ~ List.In _ [] => apply List.in_nil
+             | |- ~ List.In _ (_ :: _) => unfold not; intros
+             | H: List.In _ (_::_) |- _ => inversion H; clear H
+             | _ => discriminate
+             end.
+  Qed.
+  Next Obligation.
+    destruct x; intuition congruence.
+  Qed.
+
+  Definition states (s: state) :=
+    match s with
+    | Start =>
+      {| st_op := OpExtract 1 (HRVar Var);
+         st_trans := P4A.TSel (CExpr (EHdr (HRVar Var)))
+                              [{| sc_pat := PExact (VBits [true]);
+                                  sc_st := inl Second |};
+                              {| sc_pat := PExact (VBits [false]);
+                                 sc_st := inr true |}]
+                              (inr false) |}
+    | Second =>
+      {| st_op := OpExtract 1 (HRVar Var);
+        st_trans := P4A.TSel (CExpr (EHdr (HRVar Var)))
+                            [{| sc_pat := PExact (VBits [true]);
+                                sc_st := inl Start |};
+                            {| sc_pat := PExact (VBits [false]);
+                                sc_st := inr true |}]
+                            (inr false) |}
+    end.
+
+  Program Definition aut: Syntax.t state header :=
+    {| t_states := states |}.
+  Solve Obligations with (destruct s; cbv; Lia.lia).
+
+End LoopUnroll.
+
+Definition comb_aut := Sum.sum Loop.aut LoopUnroll.aut.
+
+(* Ltac solve_bisim' :=
+  match goal with
+  | |- pre_bisimulation _ _ _ [] _ _ =>
+    idtac "close";
+    time apply PreBisimulationClose
+  | |- pre_bisimulation _ _ _ (_ :: _) _ _ =>
+    idtac "skip";
+    time pbskip'
+  | |- pre_bisimulation ?a ?wp ?R (?C :: ?T) ?a1 ?a2 =>
+    idtac "extend";
+    let t := fresh "tmp" in
+    let Heqwp := fresh "Heqwp" in
+    let Hext := fresh "Hext" in
+    time pose (t := wp a C);
+      time assert (Heqwp: t = wp a C) by reflexivity;
+      time cbv in t;
+      time pose proof (Hext := fun R' T' pf => PreBisimulationExtend _ _ _ comb_aut (WPSymLeap.wp (H:=Sum.H Loop.header LoopUnroll.header)) R' T' C t a1 a2 Heqwp pf);
+      time unfold t in Hext;
+      time apply (Hext R T);
+      time clear Hext t Heqwp;
+      time simpl (_ ++ _) 
+  end. *)
+
+(* Lemma prebisim_loop_unroll:
+  pre_bisimulation comb_aut
+                   (WPSymLeap.wp (H:=_))
+                   nil
+                   (mk_init 10 comb_aut Loop.Start LoopUnroll.Start)
+                   (inl (inl Loop.Start), [], [])
+                   (inl (inr LoopUnroll.Start), [], []).
+Proof.
+  set (rel0 := mk_init 10 comb_aut Loop.Start LoopUnroll.Start).
+  cbv in rel0.
+  subst rel0.
+  time (repeat (time solve_bisim')).
+  cbv in *.
+  intuition (try congruence).
+Time Qed. *)
